\red{placeholder} Following the same method and reasoning as previously, however, now $d < z <h$, which gives $v(x, d, t)= u(x,d,t)= 0$ and results in $u = -\frac{\kappa}{m+1}\left( (h-d)^{m+1} - (h-z)^{m+1} \right)$
%
\begin{equation}
    Q \pd{{h}}{{t}} + Q\frac{\kappa}{m+1}\od{}{{x}}\int_d^h (h-d)^{m+1} - (h - z)^{m+1} \dif{z} = Qq
\end{equation}
which gives
\begin{equation}
    \pd{{h}}{{t}} + \frac{\kappa}{m+2}\od{}{{x}}\left[(h-d)^{m+2}\right] = q
\end{equation}
and
\begin{equation}
    v = - \pd{}{x} \frac{\kappa}{m+1} \left[ (z-d)(h-d)^{m+1} + \frac{1}{m+2} \left( [h-z]^{m+2} - (h-d)^{m+2} \right) \right].
    \label{eq:explicit_v_h}
\end{equation}